changed "EncodedType" to "EncodingType"

theories/Basics/HeterogeneousRelations.v
@@ -8,9 +8,10 @@ Require Import ITree.Basics.Basics ITree.Basics.HeterogeneousRelations.
 (* should this be polymorphic ? *)
 Universe entree_u.
 
-Class EncodedType (E : Type) := encodes : E -> Type@{entree_u}.
+(* Types that encode other types *)
+Class EncodingType (E : Type) := encodes : E -> Type@{entree_u}.
 
-#[global] Instance EncodedSum (E1 E2 : Type@{entree_u}) `{EncodedType E1} `{EncodedType E2} : EncodedType (sum E1 E2) :=
+#[global] Instance EncodingSum (E1 E2 : Type@{entree_u}) `{EncodingType E1} `{EncodingType E2} : EncodingType (sum E1 E2) :=
   fun e12 => match e12 with 
           | inl e1 => encodes e1
           | inr e2 => encodes e2 end.
@@ -20,13 +21,13 @@ Notation PostRel E1 E2 := (forall (e1 : E1) (e2 : E2), encodes e1 -> encodes e2 
 
 Notation rcompose RR1 RR2 := (rel_compose RR2 RR1).
 
-Variant SumPostRel {E1 E2 D1 D2} `{EncodedType E1} `{EncodedType E2} `{EncodedType D1} `{EncodedType D2} 
+Variant SumPostRel {E1 E2 D1 D2} `{EncodingType E1} `{EncodingType E2} `{EncodingType D1} `{EncodingType D2}
         (RPost1 : PostRel E1 E2) (RPost2 : PostRel D1 D2) : PostRel (E1 + D1) (E2 + D2) :=
   | SumPostRel_inl (e1 : E1) (e2 : E2) a b : RPost1 e1 e2 a b -> SumPostRel RPost1 RPost2 (inl e1) (inl e2) a b
   | SumPostRel_inr (d1 : D1) (d2 : D2) a b : RPost2 d1 d2 a b -> SumPostRel RPost1 RPost2 (inr d1) (inr d2) a b
 .
 
-Variant RComposePostRel {E1 E2 E3} `{EncodedType E1} `{EncodedType E2} `{EncodedType E3}
+Variant RComposePostRel {E1 E2 E3} `{EncodingType E1} `{EncodingType E2} `{EncodingType E3}
         (RPre1 : Rel E1 E2) (RPre2 : Rel E2 E3) (RPost1 : PostRel E1 E2) (RPost2 : PostRel E2 E3) : PostRel E1 E3 :=
   | RComposePostRel_intro (e1 : E1) (e3 : E3) a c : 
     (forall e2, RPre1 e1 e2 -> RPre2 e2 e3 -> exists b, RPost1 e1 e2 a b /\ RPost2 e2 e3 b c) ->
