theories/Core/SubEvent.v
@@ -9,22 +9,22 @@ Require Import HeterogeneousRelations EnTreeDefinition.
 
 Class ReSum (E1 E2 : Type) : Type := resum : E1 -> E2.
 
-Class ReSumRet E1 E2 `{EncodedType E1} `{EncodedType E2} `{ReSum E1 E2} : Type :=
+Class ReSumRet E1 E2 `{EncodingType E1} `{EncodingType E2} `{ReSum E1 E2} : Type :=
   resum_ret : forall (e : E1), encodes (resum e) -> encodes e.
 
 #[global] Instance ReSum_inl E1 E2 : ReSum E1 (E1 + E2) := inl.
 #[global] Instance ReSum_inr E1 E2 : ReSum E2 (E1 + E2) := inr.
-#[global] Instance ReSumRet_inl E1 E2 `{EncodedType E1} `{EncodedType E2} : ReSumRet E1 (E1 + E2) :=
+#[global] Instance ReSumRet_inl E1 E2 `{EncodingType E1} `{EncodingType E2} : ReSumRet E1 (E1 + E2) :=
   fun _ e => e.
-#[global] Instance ReSumRet_inr E1 E2 `{EncodedType E1} `{EncodedType E2} : ReSumRet E2 (E1 + E2) :=
+#[global] Instance ReSumRet_inr E1 E2 `{EncodingType E1} `{EncodingType E2} : ReSumRet E2 (E1 + E2) :=
   fun _ e => e.
 
-Definition trigger {E1 E2 : Type} `{EncodedType E1} `{EncodedType E2} `{ReSum E1 E2} `{ReSumRet E1 E2} 
+Definition trigger {E1 E2 : Type} `{EncodingType E1} `{EncodingType E2} `{ReSum E1 E2} `{ReSumRet E1 E2}
            (e : E1) : entree E2 (encodes e) :=
   Vis (resum e) (fun x : encodes (resum e) => Ret (resum_ret e x)).
 
 (* Use resum and resum_ret to map the events in an entree to another type *)
-CoFixpoint resumEntree {E1 E2 : Type} `{EncodedType E1} `{EncodedType E2}
+CoFixpoint resumEntree {E1 E2 : Type} `{EncodingType E1} `{EncodingType E2}
            `{ReSum E1 E2} `{ReSumRet E1 E2} A (t : entree E1 A) : entree E2 A :=
   match observe t with
   | RetF r => Ret r
